Comment on propositions in paper, reorg aeq properties, add vrel properties
* Fixes #17: Add comments pointing to equivalent propositions in paper
* Fixes #18: Rename vrel.combined to vrel.properties

src/aeq/id.lean
@@ -4,7 +4,7 @@ This file contains declarations related to `aeq` identity or reflexivity.
 
 -/
 
-import .map
+import .properties
 
 namespace acie ----------------------------------------------------------------
 namespace aeq ------------------------------------------------------------------
@@ -13,29 +13,35 @@ variables {V : Type} [decidable_eq V] -- Type of variable names
 variables {vs : Type → Type} [vset vs V] -- Type of variable name sets
 variables {X : vs V} -- Variable name sets
 
--- Identity of one expression
-protected
-def id (e : exp X) : e ≡α e :=
-  begin
-    induction e with
-      /- var -/ X x
-      /- app -/ X f e rf re
-      /- lam -/ X a e r,
-    begin /- var -/
-      exact var (vrel.refl x)
-    end,
-    begin /- app -/
-      exact app rf re
-    end,
-    begin /- lam -/
-      exact lam (map.simple (λ x y, vrel.update.of_id) r)
-    end
-  end
+-- Identity `aeq` with an implicit `vset`.
+@[inline, reducible]
+def aeq.id {X : vs V} : exp X → exp X → Prop :=
+  aeq (vrel.id X)
 
--- Reflexivity
+-- Notation for `aeq.id`.
+infix ` ≡α `:50 := aeq.id
+
+namespace id -------------------------------------------------------------------
+-- Paper: Corollary 3
+
+-- Reflexivity of `aeq.id`
 protected
-theorem refl (X : vs V) : reflexive (aeq.identity X) :=
-  aeq.id
+theorem refl (X : vs V) : reflexive (aeq (vrel.id X)) :=
+  aeq.refl
+
+-- Symmetry of `aeq.id`
+protected
+theorem symm (X : vs V) : symmetric (aeq (vrel.id X)) :=
+  λ e₁ e₂ a,
+  map.simple (λ x₁ x₂, vrel.inv.of_id) (aeq.symm a)
+
+-- Transitivity of `aeq.id`
+protected
+theorem trans (X : vs V) : transitive (aeq (vrel.id X)) :=
+  λ e₁ e₂ e₃ a₁ a₂,
+  map.simple (λ x₁ x₂, vrel.id.of_comp) (aeq.trans a₁ a₂)
+
+end /- namespace -/ id ---------------------------------------------------------
 
 end /- namespace -/ aeq --------------------------------------------------------
 end /- namespace -/ acie ------------------------------------------------------
