src/aeq/default.lean
@@ -1,5 +1,5 @@
 import .type
 import .map
+import .properties
 import .id
-import .inv
 import .subst
